Fix

CpcMini/SmtModel.lean
@@ -384,10 +384,15 @@ def native_veq : SmtValue -> SmtValue -> native_Bool
     (typeofValue : SmtValue -> SmtType)
     (valueEq : SmtType -> SmtValue -> SmtValue -> native_Bool) :
     SmtValue -> SmtValue -> native_Nat -> native_Bool
-  | (SmtValue.Apply f1 v1), (SmtValue.Apply f2 v2), native_nat_succ n =>
-      native_and (native_apply_veq typeofValue valueEq f1 f2 n)
-        (native_apply_veq typeofValue valueEq v1 v2 n)
-  | v1, v2, _ => valueEq (typeofValue v1) v1 v2
+  | (SmtValue.Apply f1 v1), (SmtValue.Apply f2 v2), _ =>
+      native_and (native_apply_veq typeofValue valueEq f1 f2 native_nat_zero)
+        (native_apply_veq typeofValue valueEq v1 v2 native_nat_zero)
+  | v1, v2, _ =>
+      native_and (native_Teq (typeofValue v1) (typeofValue v2))
+        (valueEq (typeofValue v1) v1 v2)
+termination_by v1 v2 _ => sizeOf v1 + sizeOf v2
+decreasing_by
+  all_goals subst_vars; simp_wf; omega
 
 macro_rules
   | `(native_veq_ext $T $U $m1 $m2) => do
@@ -496,12 +501,21 @@ def __vsm_apply_arg_nth : SmtValue -> native_Nat -> native_Nat -> SmtValue
 
 
 def __smtx_value_eq : SmtType -> SmtValue -> SmtValue -> native_Bool
-  | (SmtType.Map T1 T2), (SmtValue.Map m1), (SmtValue.Map m2) => (native_veq_ext T1 T2 m1 m2)
-  | (SmtType.Set T1), (SmtValue.Set m1), (SmtValue.Set m2) => (native_veq_ext T1 SmtType.Bool m1 m2)
-  | (SmtType.FunType T1 T2), (SmtValue.Fun m1), (SmtValue.Fun m2) => (native_veq_ext T1 T2 m1 m2)
-  | SmtType.RegLan, (SmtValue.RegLan r1), (SmtValue.RegLan r2) => (native_re_ext_eq r1 r2)
-  | (SmtType.Seq T), (SmtValue.Seq (SmtSeq.empty T1)), (SmtValue.Seq (SmtSeq.empty T2)) => true
-  | (SmtType.Seq T), (SmtValue.Seq (SmtSeq.cons v1 vs1)), (SmtValue.Seq (SmtSeq.cons v2 vs2)) => (native_and (__smtx_value_eq T v1 v2) (__smtx_value_eq (SmtType.Seq T) (SmtValue.Seq vs1) (SmtValue.Seq vs2)))
+  | (SmtType.Map T U), (SmtValue.Map m1), (SmtValue.Map m2) =>
+      (native_veq_ext T U m1 m2)
+  | (SmtType.Set T), (SmtValue.Set m1), (SmtValue.Set m2) =>
+      (native_veq_ext T SmtType.Bool m1 m2)
+  | (SmtType.FunType T U), (SmtValue.Fun m1), (SmtValue.Fun m2) =>
+      (native_veq_ext T U m1 m2)
+  | SmtType.RegLan, (SmtValue.RegLan r1), (SmtValue.RegLan r2) =>
+      (native_re_ext_eq r1 r2)
+  | (SmtType.Seq T), (SmtValue.Seq (SmtSeq.empty T1)),
+      (SmtValue.Seq (SmtSeq.empty T2)) => true
+  | (SmtType.Seq T), (SmtValue.Seq (SmtSeq.cons v1 vs1)),
+      (SmtValue.Seq (SmtSeq.cons v2 vs2)) =>
+      (native_and (__smtx_value_eq T v1 v2)
+        (__smtx_value_eq (SmtType.Seq T) (SmtValue.Seq vs1)
+          (SmtValue.Seq vs2)))
   | T, v1, v2 => (native_veq v1 v2)
 termination_by
   T v1 v2 => (sizeOf T, 0, sizeOf v1 + sizeOf v2)
